%!TEX root =  bgo.tex
% please do not delete or change the first line (needed by Csaba's editor)

Before the proof, we introduce a well known bound on the instantaneous linearized regret of Mirror Descent. \todox{Should add some citation, but I can not find a proper source.}
\begin{lemma}
\label{lem:mdlinregret}
For any $x \in \cK$ and any $t \ge 1$,
\begin{align*}
\MoveEqLeft
\ip{G_t, X_{t+1}-x} \\
\le &\dfrac{1}{\eta_t} \left( \DR(x,X_t)-\DR(x,X_{t+1})-\DR(X_{t+1},X_t) \right)\,,
\end{align*}
where $X_{t+1}$ is selected as in \cref{alg}.
\end{lemma}
\begin{proof}
The point $X_{t+1}$ is the minimizer of 
$\Psi_{t+1}(x)=\eta_t \ip{G_t,x}+\DR(x,X_t)$ over $\cK$. The gradient of $\Psi_{t+1}(x)$ is
\[
\nabla \Psi_{t+1}(x) = \eta_t G_t + \nabla\mathcal{R}(x)-\nabla\mathcal{R}(X_t)\,.
\]
By the optimality condition, for any $x \in \cK$,
\[
\ip{\eta_t G_t + \nabla\mathcal{R}(x)-\nabla\mathcal{R}(X_t), x-X_{t+1}}\ge 0 \,,
\]
which is equivalent to the result by substituting the definition of Bregman divergence $\DR$.
\end{proof}

Proof of Lemma \ref{lem:ub}:

Denote $\hat{G}_t = \nabla f(X_t)$. 
From the smoothness and convexity of $f$ and using that $\mathcal{R}$ is strongly convex, we have
\begin{align}
\MoveEqLeft
f(X_{t+1}) - f(x) \nonumber\\
 \le& f(X_t) + \ip{ \hat{G}_t, X_{t+1}-X_t } + \frac{L}{2} \norm{X_{t+1}-X_t}^2 \nonumber \\
&- \left\{ f(X_t) + \ip{ \hat{G}_t, x-X_t} \right\} \nonumber \\
 =& \ip{\hat{G}_t, X_{t+1} - x } +  \frac{L}{2} \norm{X_{t+1}-X_t}^2 \nonumber\\
 \le& \ip{\hat{G}_t,X_{t+1}-x} + \frac{L}{\alpha} D_{\mathcal{R}}(X_{t+1},X_t)\,. \label{eq:mdsmoothnoisy1}
\end{align}
Now write $\hat{G}_t = (\hat{G}_t-\overline G_t)  + \xi_t + G_t$ where $\xi_t = \overline G_t - G_t$ is the ``noise''.
Hence, 
\begin{align*}
\MoveEqLeft
\ip{\hat{G}_t,X_{t+1}-x} \\
\le& \beta_t \norm{X_{t+1}-x} + \ip{\xi_t,X_{t+1}-x} + \ip{ G_t, X_{t+1} - x }\\
\le &\beta_t \sqrt{ \frac{2D}{\alpha} } + \ip{\xi_t,X_{t+1}-x} + \ip{ G_t, X_{t+1} - x } \,.
\end{align*}
After we plug this into~\eqref{eq:mdsmoothnoisy1},
the plan is to take the conditional expectation of both sides w.r.t. $\F_{t}$.
As $X_t$ is $\F_{t}$-measurable, and by the definition of $\xi_t$ and $\overline G_t$, $\EE{ \xi_t|\F_{t}} = 0$, 
we have 
\begin{align*}
\MoveEqLeft
\EE{\ip{\xi_t, X_{t+1}-x}|\F_{t}} \\
&= \underbrace{\EE{\ip{\xi_t,X_{t}-x}|\F_{t}}}_{=0} + \EE{\ip{\xi_t,X_{t+1}-X_t}|\F_{t}} \,.
\end{align*}
We bound the second term inside the expectation from the Fenchel-Young inequality: 
\begin{align*}
\ip{\xi_t,X_{t+1}-X_t} \le \frac12 \left(\frac{\norm{\xi_t}_*^2}{a_t} + a_t \norm{X_{t+1}-X_t}^2\right)\,.
\end{align*}
Using again that $\mathcal{R}$ is $\alpha$-strongly convex, we get 
\[
\ip{\xi_t,X_{t+1}-X_t} \le \frac12 \left(\frac{\norm{\xi_t}_*^2}{a_t} + \frac{2a_t}{\alpha} D_{\mathcal{R}}(X_{t+1},X_t) \right)\,.
\]
Applying 
\cref{lem:mdlinregret} 
to bound $\ip{ G_t, X_{t+1} - x }$, and putting everything together gives
\begin{align*}
\MoveEqLeft \EE{f(X_{t+1}) - f(x) |\F_{t} }
\le 
 \beta_t \sqrt{ \frac{2D}{\alpha} }+
\frac{1}{2a_t}  \EE{\norm{\xi_t}_*^2|\F_{t}}\\&+
\frac{1}{\eta_t} \left(D_{\mathcal{R}}(x,X_t)-D_{\mathcal{R}}(x,X_{t+1})\right) \\&+
\underbrace{\left(\frac{a_t+L}{\alpha}-\frac{1}{\eta_t}\right) D_{\mathcal{R}}(X_{t+1},X_t)}_{=0} \,.
\end{align*}
Given $\sigma_t^2 = \EE{ \norm{\xi_t}_*^2}$,
we will sum up these inequalities for $t=1,\dots,n-1$.
To bound the right-hand side of the result, we use
\begin{align*}
\MoveEqLeft \sum_{t=1}^{n-1} \frac{1}{\eta_t} \left(\DR(x,X_t)-\DR(x,X_{t+1})\right)
 \\
&= \DR(x,X_1) \frac{1}{\eta_1} + \DR(x,X_2) \left(\frac{1}{\eta_2}-\frac{1}{\eta_1}\right)
+ \dots  \\
& \dots+\DR(x,X_{n-1}) \left(\frac{1}{\eta_{n-1}} -\frac{1}{\eta_{n-2}}\right)\\
&- \frac{1}{\eta_{n-1}} \DR(x,X_n)\\
& \le D \frac{1}{\eta_1} + D \sum_{t=2}^{n-1} \left(\frac1{\eta_{t}}-\frac1{\eta_{t-1}}\right)\\
& = \frac{D}{\eta_{n-1}}\,.
\end{align*}
The inequality results from the fact that $\{\eta_t\}$ is non-increasing.
Hence, by the tower rule,
\begin{align*}
 &\EE{ \sum_{t=1}^n f(X_t) - f(x) }  \\
\le& 
  \EE{f(X_1)-f(x)} + \sqrt{\tfrac{2D}{\alpha}} \sum_{t=1}^{n-1} \beta_t +
	   \frac{D}{\eta_{n-1}} +
	  \sum_{t=1}^{n-1}\frac{\sigma_t^2}{2a_t}\\
=& 	  
  \EE{f(X_1)-f(x)} + \sqrt{\tfrac{2D}{\alpha}} \sum_{t=1}^{n-1} \beta_t +
	   \frac{D(a_{n-1}+L)}{\alpha} +
	  \sum_{t=1}^{n-1}\frac{\sigma_t^2}{2a_t}\,.
\end{align*}