%!TEX root =  bgo.tex
% please do not delete or change the first line (needed by Csaba's editor)
\subsection{Reductions and Proofs}
\label{sec:orrel}

\begin{theorem}
\cref{def:oracle1} is a sufficient condition of \cref{def:oracle2}, given a bounded $\cK$. That is, for any $(c_1,c_2)$ Type-I oracle $\gamma$, there exist some constant $R$ such that  $\gamma$ is a $(c'_1,c_2)$ Type-II oracle, with $c'_1(\delta)=Rc_1(\delta)$.

Similarly, \cref{def:oracle2} is sufficient for \cref{def:oracle1} if the alternative condition \eqref{eq:oracle2alt} holds.
\end{theorem}
\begin{proof}
Given $\norm{ \EE{G}  - \nabla f(x)  }_* \le c_1(\delta) $ in \cref{def:oracle1}, we can always construct a function $\tilde{f}:\cK \to \mathbb{R}$, 
\[
\tilde{f}(y) =\EE{ f(y)+ \left( G-\nabla f(x) \right)^\top y} \,, 
\]
where the expection is over the randomness of $G$, satisfying
\begin{align*}
\MoveEqLeft
\norm{\tilde{f}(y)-f(y)}_{\infty} \\
= &
 \norm{ \EE{\left( G-\nabla f(x) \right)^\top y}}_{\infty}\\
 \le &\norm{\EE{G}-\nabla f(x)}_* \norm{y}
 \le  Rc_1(\delta)\,,
\end{align*} 
by choosing $R = \sup_{y \in \cK}\norm{y}$.

Also notice that
\[
 \nabla \tilde{f}(x) = \EE{\nabla f(x)+ \left( G-\nabla f(x)\right)}
 =\EE{G}\,.
\]
Therefore, $\gamma$ is also a $(c'_1,c_2)$ Type-II oracle.

Next, given \eqref{eq:oracle2alt} and $\EE{G}=\nabla \tilde{f}(x)$ in \cref{def:oracle2}, we can immediately get the bias condition of \cref{def:oracle1}. \todox{should add an inequality $\norm{\cdot}_* \le C \norm{\cdot}_\infty$}
\end{proof}

